\documentclass[11pt, paper=a4]{article}
\usepackage[left=4.5cm, right=4.5cm, %showframe
]{geometry}

\usepackage{amsmath}
\usepackage{amsthm}       
\usepackage{amssymb} 

\newcommand{\E}{\operatorname{\mathbf{E}}}
\newcommand{\Var}{\operatorname{\mathbf{Var}}}

\addtolength{\parskip}{\baselineskip}
\parindent 0pt

\begin{document}

\section*{S1}

Solving
\begin{align}
\mu = px + (1-p)y
\end{align}
for $p$ gives
\begin{align}
  p = \frac{\mu-y}{x-y},
\end{align}
%
which, plugged into
\begin{align}
  \varrho = \frac{p x^2 + (1-p) y^2}{\mu^2},
\end{align}
yields
\begin{align}
  \varrho & = \frac{\left(\frac{\mu-y}{x-y}\right)x^2  + \left(1-\frac{\mu-y}{x-y}\right) y^2}{\mu^2} \\ & = \underbrace{\frac{(\mu - y)x^2}{(x-y)\mu^2}}_{\mathrm{(I)}}\,\, + \,\, \underbrace{\frac{y^2}{\mu^2}}_{\mathrm{(II)}}\,\, - \,\, \underbrace{\frac{(\mu - y)y^2}{(x-y) \mu^2}}_{\mathrm{(III)}}.
\end{align}

The summands are
\begin{align}
  \mathrm{(I):} \quad & \frac{(\mu - y)x^2}{(x-y)\mu^2} = \frac{x^2}{(x-y)\mu} - \frac{yx^2}{(x-y)\mu^2} \\
  \mathrm{(II):} \quad &  \frac{y^2}{\mu^2} = \frac{(x-y)y^2}{(x-y)\mu^2} = \frac{xy^2}{(x-y)\mu^2} - \frac{y^3}{(x-y)\mu^2} \\
  \mathrm{(III):} \quad & - \frac{(\mu - y)y^2}{(x-y) \mu^2} = \frac{y^3}{(x-y)\mu^2} - \frac{y^2}{(x-y)\mu}
\end{align}

Putting everything together we get
\begin{align}
  \varrho & =  \frac{x^2 - y^2}{(x-y)\mu} + \frac{xy^2 -yx^2}{(x-y)\mu^2}  = \frac{(x + y) (x-y)}{(x-y)\mu} - \frac{xy (x-y)}{(x-y)\mu^2} \\
  & = \frac{x+y}{\mu} - \frac{xy}{\mu^2}.
\end{align}

\section*{S2}
Solve
\begin{align}
  p = \frac{\mu-y}{x-y}
\end{align}
for $y$ and since $x \geq \mu$,
\begin{align}
y = \frac{\mu - px}{1-p} \leq \frac{\mu - p\mu}{1-p} = \mu.
\end{align}
\end{document}
